\begin{matrix}
\text{Quadratic\ Equation} & {x = \frac{- b \pm \sqrt{b_{}^{2} - 4ac}}{2a}} \\
\text{DisplayQuadratic\ Equation} & {x = \frac{- b \pm \sqrt{b_{}^{2} - 4ac}}{2a}} \\
\text{Rational\ Function} & {f(x) = \frac{1 - x_{}^{2}}{1 - x_{}^{3}}} \\
\text{Rational\ Function} & {f(x) = \frac{(1 - x_{}^{2})x_{}^{3}}{1 - x_{}^{3}}} \\
\text{Rational\ Function} & {f(x) = \frac{(1 - x_{}^{2})(x_{}^{3} - 5x)}{1 - x_{}^{3}}} \\
\text{Parametrize\ Rational\ Function} & {f(x) = \frac{(a_{i}^{} - x_{}^{2})_{}^{5}}{1 - x_{}^{3}}} \\
\text{Stacked\ exponents} & {g(z) = e_{}^{- x_{}^{2}}} \\
\text{Stacked\ exponents} & {g(z) = e_{}^{- (z - a)_{}^{2}}} \\
\text{Stacked\ exponents} & {g(z) = e_{}^{- \sum\limits_{i = 0}^{\infty}z_{i}^{2}}} \\
\text{Stacked\ exponents} & {g(y) = e_{}^{- \sum\limits_{i = 0}^{\infty}y_{i}^{2}}} \\
\text{Stacked\ exponents} & {g(z) = e_{}^{- \sum\limits_{i = 0}^{\infty}z_{}^{\frac{2}{a - i}}}} \\
\text{Cross\ Product} & {\frac{x_{1}^{} - x_{2}^{}}{x_{3}^{} - x_{4}^{}}\frac{x_{1}^{} - x_{4}^{}}{x_{2}^{} - x_{3}^{}}} \\
\text{Cross\ Product} & {(\frac{x_{1}^{} - x_{2}^{}}{x_{3}^{} - x_{4}^{}})(\frac{x_{1}^{} - x_{4}^{}}{x_{2}^{} - x_{3}^{}})} \\
\text{Cross\ Product} & {\left( \frac{x_{1}^{} - x_{2}^{}}{x_{3}^{} - x_{4}^{}} \right)\left( \frac{x_{1}^{} - x_{4}^{}}{x_{2}^{} - x_{3}^{}} \right)} \\
\text{Cross\ Product} & \frac{(x_{1}^{} - x_{2}^{})(x_{3}^{} - x_{4}^{})}{(x_{1}^{} - x_{4}^{})(x_{2}^{} - x_{3}^{})} \\
\end{matrix}
